Phi_Examples/Rational_Arith.thy
@@ -7,7 +7,7 @@ abbreviation \<open>\<r>\<a>\<t>\<i>\<o>\<n>\<a>\<l> \<equiv> \<struct>{num: \<a
 
   
 \<phi>type_def \<phi>Rational ("\<rat>")
-  where \<open>x \<Ztypecolon> \<phi>Rational \<equiv> (n,d) \<Ztypecolon> \<lbrace> num: \<int>, den: \<int> \<rbrace> \<subj> n d. of_int n / of_int d = x \<and> d \<noteq> 0\<close>
+  where \<open>(x::rat) \<Ztypecolon> \<phi>Rational \<equiv> (n,d) \<Ztypecolon> \<lbrace> num: \<int>, den: \<int> \<rbrace> \<subj> n d. of_int n / of_int d = x \<and> d \<noteq> 0\<close>
   deriving Basic
        and \<open>Object_Equiv \<rat> (=)\<close>
        and \<open>Abstract_Domain\<^sub>L \<rat> (\<lambda>_. True)\<close>
